Working on reductions

src/Reduction.v
@@ -2,6 +2,8 @@ Require Import Bool List String Peano_dec.
 Require Import Common ListSupport FMap Syntax Semantics StepM SemFacts.
 Require Import Serial.
 
+Require Import Permutation.
+
 Set Implicit Arguments.
 
 Ltac dest_step_m :=
@@ -26,9 +28,19 @@ Definition InternalHistory (hst: MHistory) :=
 Definition Reduced (sys: System) (hfr hto: MHistory) :=
   forall st1 st2,
     steps step_m sys st1 hfr st2 ->
-    steps step_m sys st1 hto st2.
+    steps step_m sys st1 hto st2 /\
+    BEquivalent sys hfr hto.
 
 (*! General Facts *)
+
+Lemma internal_history_behavior_nil:
+  forall sys hst,
+    InternalHistory hst -> behaviorOf sys hst = nil.
+Proof.
+  induction hst; simpl; intros; auto.
+  inv H; rewrite IHhst by assumption.
+  destruct a; auto; elim H2.
+Qed.
 
 Lemma reduced_app_1:
   forall sys hfr hto,
@@ -38,7 +50,11 @@ Lemma reduced_app_1:
 Proof.
   unfold Reduced; intros.
   eapply steps_split in H0; [|reflexivity]; dest.
-  eapply steps_append; eauto.
+  specialize (H _ _ H0); dest.
+  split.
+  - eapply steps_append; eauto.
+  - red; do 2 rewrite behaviorOf_app.
+    rewrite H2; reflexivity.
 Qed.
 
 Lemma reduced_app_2:
@@ -49,15 +65,28 @@ Lemma reduced_app_2:
 Proof.
   unfold Reduced; intros.
   eapply steps_split in H0; [|reflexivity]; dest.
-  eapply steps_append; eauto.
+  specialize (H _ _ H1); dest.
+  split.
+  - eapply steps_append; eauto.
+  - red; do 2 rewrite behaviorOf_app.
+    rewrite H2; reflexivity.
 Qed.
 
-(* Lemma reduced_serializable: *)
-(*   forall sys hfr, *)
-(*     Serializable sys hfr -> *)
-(*     forall hto, *)
-(*       Reduced sys hfr hto -> *)
-(*       Serializable sys hto. *)
+Lemma reduced_serializable:
+  forall sys st1 hfr st2,
+    steps step_m sys st1 hfr st2 ->
+    Serializable sys hfr ->
+    forall hto,
+      Reduced sys hfr hto ->
+      Serializable sys hto.
+Proof.
+  unfold Serializable, Reduced; intros.
+  destruct H0 as [shfr [stfr [? ?]]].
+  exists shfr, stfr.
+  split; auto.
+  specialize (H1 _ _ H); dest.
+  congruence.
+Qed.
 
 (*! Facts to prove serializability *)
 
@@ -67,97 +96,161 @@ Lemma msg_ins_commutes:
     Reduced sys [RlblIns eins; lbl] [lbl; RlblIns eins].
 Proof.
   unfold Reduced; intros.
-  destruct lbl as [|hdl mins mouts|]; [elim H| |elim H].
-  dest_step_m.
-  - econstructor.
+  split.
+  - destruct lbl as [|hdl mins mouts|]; [elim H| |elim H].
+    dest_step_m.
     + econstructor.
-      * econstructor. 
-      * econstructor; eauto. 
+      * econstructor.
+        { econstructor. } 
+        { econstructor; eauto. }
+      * econstructor.
     + econstructor.
-  - econstructor.
-    + econstructor.
-      * econstructor. 
-      * econstructor; eauto. 
-    + econstructor; try reflexivity; try eassumption.
-      * clear -H9; induction mins; simpl; [constructor|].
-        inv H9; constructor; auto.
-        apply FirstMP_enqMsgs; auto.
-      * f_equal.
-        admit. (* requires a lemma about [MessagePool] *)
-Admitted.
+      * econstructor.
+        { econstructor. }
+        { econstructor; eauto. }
+      * econstructor; try reflexivity; try eassumption.
+        { eapply FirstMPI_Forall_enqMsgs; eauto. }
+        { f_equal.
+          rewrite enqMsgs_enqMsgs_comm.
+          { rewrite enqMsgs_deqMsgs_FirstMPI_comm; auto.
+            destruct H10; auto.
+          }
+          { destruct H2, H17.
+            eapply DisjList_SubList; eauto.
+            eapply DisjList_comm, DisjList_SubList; eauto.
+            apply DisjList_app_4.
+            { apply mindsOf_merqsOf_DisjList. }
+            { apply DisjList_comm, merqsOf_merssOf_DisjList. }
+          }
+        }
+  - hnf; cbn.
+    destruct lbl; [elim H|auto|elim H].
+Qed.
 
 Lemma msg_in_reduced:
   forall sys eins hst2,
     InternalHistory hst2 ->
     Reduced sys (RlblIns eins :: hst2) (hst2 ++ [RlblIns eins]).
 Proof.
-  unfold Reduced; induction hst2 as [|lbl ?]; simpl; intros; auto.
+  unfold Reduced; induction hst2 as [|lbl ?]; simpl; intros;
+    [split; [assumption|reflexivity]|].
   inv H.
-  change (RlblIns eins :: lbl :: hst2) with ([RlblIns eins; lbl] ++ hst2) in H0.
-  eapply steps_split in H0; [|reflexivity].
-  destruct H0 as [sti [? ?]].
-  eapply msg_ins_commutes in H0; [|assumption].
-  pose proof (steps_append H H0); inv H1.
-  specialize (IHhst2 H4 _ _ H7).
-  econstructor; eauto.
+  split.
+  - change (RlblIns eins :: lbl :: hst2) with ([RlblIns eins; lbl] ++ hst2) in H0.
+    eapply steps_split in H0; [|reflexivity].
+    destruct H0 as [sti [? ?]].
+    eapply msg_ins_commutes in H0; [|assumption]; dest.
+    pose proof (steps_append H H0); inv H2.
+    specialize (IHhst2 H4 _ _ H8); dest.
+    econstructor; eauto.
+  - red; cbn.
+    rewrite behaviorOf_app.
+    rewrite internal_history_behavior_nil by assumption.
+    destruct lbl; auto; elim H3.
 Qed.
 
 Lemma msg_outs_commutes:
-  forall sys st1 eouts lbl st2,
+  forall sys eouts lbl,
     Internal lbl ->
-    steps step_m sys st1 [lbl; RlblOuts eouts] st2 ->
-    steps step_m sys st1 [RlblOuts eouts; lbl] st2.
+    Reduced sys [lbl; RlblOuts eouts] [RlblOuts eouts; lbl].
 Proof.
-  intros.
-  destruct lbl as [|hdl mins mouts|]; [elim H| |elim H].
-  dest_step_m.
-  - econstructor.
+  unfold Reduced; intros.
+  split.
+  - destruct lbl as [|hdl mins mouts|]; [elim H| |elim H].
+    dest_step_m.
     + econstructor.
-      * econstructor. 
-      * econstructor; eauto. 
-    + econstructor; eauto.
-  - econstructor.
+      * econstructor.
+        { econstructor. }
+        { econstructor; eauto. }
+      * econstructor; eauto.
     + econstructor.
-      * econstructor. 
-      * econstructor; try reflexivity; try eassumption.
-        admit. (* requires a lemma about [MessagePool] *)
-    + econstructor; try reflexivity; try eassumption.
-      * admit. (* requires a lemma about [MessagePool] *)
-      * f_equal.
-        admit. (* requires a lemma about [MessagePool] *)
-Admitted.
+      * econstructor.
+        { econstructor. }
+        { econstructor; try reflexivity; try eassumption.
+          assert (DisjList (idsOf mins) (idsOf eouts)).
+          { destruct H3, H12.
+            eapply DisjList_SubList; eauto.
+            eapply DisjList_comm, DisjList_SubList; eauto.
+            apply DisjList_comm, mindsOf_merssOf_DisjList.
+          }
+          eapply FirstMPI_Forall_deqMsgs; eauto.
+        }
+      * assert (DisjList (idsOf eouts) (idsOf mins)).
+        { destruct H3, H12.
+          eapply DisjList_SubList; eauto.
+          eapply DisjList_comm, DisjList_SubList; eauto.
+          apply mindsOf_merssOf_DisjList.
+        }
+        econstructor; try reflexivity; try eassumption.
+        { eapply FirstMPI_Forall_enqMsgs.
+          rewrite <-FirstMPI_Forall_deqMsgs; eauto.
+        }
+        { f_equal; rewrite <-enqMsgs_deqMsgs_FirstMPI_comm.
+          { f_equal; eapply deqMsgs_deqMsgs_comm.
+            apply DisjList_comm; auto.
+          }
+          { destruct H3; auto. }
+          { rewrite <-FirstMPI_Forall_deqMsgs; eauto. }
+        }
+  - hnf; cbn.
+    destruct lbl; [elim H|auto|elim H].
+Qed.
 
 Lemma msg_outs_reduced:
-  forall sys st1 eouts hst2 st2,
-    steps step_m sys st1 (hst2 ++ [RlblOuts eouts]) st2 ->
+  forall sys eouts hst2,
     InternalHistory hst2 ->
-    steps step_m sys st1 (RlblOuts eouts :: hst2) st2.
+    Reduced sys (hst2 ++ [RlblOuts eouts]) (RlblOuts eouts :: hst2).
 Proof.
-  induction hst2 as [|lbl ?]; simpl; intros; auto.
+  unfold Reduced; induction hst2 as [|lbl ?]; simpl; intros; 
+    [split; [assumption|reflexivity]|].
   inv H0; inv H.
-  specialize (IHhst2 _ H5 H4).
-  assert (steps step_m sys st1 (lbl :: RlblOuts eouts :: hst2) st2)
-    by (econstructor; eauto).
-  change (lbl :: RlblOuts eouts :: hst2) with
-      ([lbl; RlblOuts eouts] ++ hst2) in H.
-  eapply steps_split in H; [|reflexivity].
-  destruct H as [sti [? ?]].
-  change (RlblOuts eouts :: lbl :: hst2) with
-      ([RlblOuts eouts; lbl] ++ hst2).
-  eapply steps_append; eauto.
-  eapply msg_outs_commutes; eauto.
+  split.
+  - specialize (IHhst2 H3 _ _ H4); dest.
+    assert (steps step_m sys st1 (lbl :: RlblOuts eouts :: hst2) st2)
+      by (econstructor; eauto).
+    change (lbl :: RlblOuts eouts :: hst2) with
+        ([lbl; RlblOuts eouts] ++ hst2) in H1.
+    eapply steps_split in H1; [|reflexivity].
+    destruct H1 as [sti [? ?]].
+    change (RlblOuts eouts :: lbl :: hst2) with
+        ([RlblOuts eouts; lbl] ++ hst2).
+    eapply steps_append; eauto.
+    eapply msg_outs_commutes; eauto.
+  - red; cbn.
+    rewrite behaviorOf_app.
+    rewrite internal_history_behavior_nil by assumption.
+    destruct lbl; auto; elim H2.
 Qed.
 
-Lemma msg_outs_reduced_app:
-  forall sys st1 hst1 eouts hst2 st2,
-    steps step_m sys st1 (hst1 ++ hst2 ++ [RlblOuts eouts]) st2 ->
-    InternalHistory hst2 ->
-    steps step_m sys st1 (hst1 ++ RlblOuts eouts :: hst2) st2.
+Lemma msg_int_commutes_1:
+  forall sys rule1 ins1 outs1 rule2 ins2 outs2,
+    Reduced sys [RlblInt rule2 ins2 outs2; RlblInt rule1 ins1 outs1]
+            [RlblInt rule1 ins1 outs1; RlblInt rule2 ins2 outs2].
 Proof.
-  intros.
-  eapply steps_split in H; [|reflexivity].
-  destruct H as [sti [? ?]].
-  eapply msg_outs_reduced in H; eauto.
-  eapply steps_append; eauto.
-Qed.
+Admitted.
 
+Lemma msg_int_commutes_2:
+  forall sys rule1 ins1 outs1 rule2 ins2 outs2 rule3 ins3 outs3,
+    Reduced sys [RlblInt rule3 ins3 outs3;
+                   RlblInt rule2 ins2 outs2;
+                   RlblInt rule1 ins1 outs1]
+            [RlblInt rule3 ins3 outs3;
+               RlblInt rule1 ins1 outs1;
+               RlblInt rule2 ins2 outs2].
+Proof.
+Admitted.
+
+(* Lemma msg_int_commutes_2: *)
+(*   forall sys eins lbl, *)
+(*     Internal lbl -> *)
+(*     Reduced sys [RlblIns eins; lbl] [lbl; RlblIns eins]. *)
+(* Proof. *)
+
+
+(* Theorem request_forwardings_reduced: *)
+(*   forall rqr rqin rqfwds hsts, *)
+(*     Forall (fun rqhst => exists houts, Atomic (fst rqhst) (snd rqhst) houts) *)
+(*            (combine rqfwds hsts) -> *)
+(*     forall sys indeps, *)
+(*       Reduced sys (List.concat (indeps ++ hsts) ++ [RlblInt rqr [rqin] rqfwds]) *)
+(*               nil. (* TODO *) *)
