src/Topology.v
@@ -3,80 +3,92 @@ Require Import Common FMap.
 
 Set Implicit Arguments.
 
-Section Tree.
+(** Tree structure with (possibly-)multiple channels between nodes. *)
+Section CTree.
   Variable (t: Type).
 
-  Inductive Tree :=
-  | Node: IdxT -> t -> list Tree -> Tree.
+  Record Channel :=
+    { chn_up: list IdxT;
+      chn_down: list IdxT
+    }.
 
-  Fixpoint trIndicesOf (tr: Tree) :=
+  Inductive CTree :=
+  | CNode: IdxT -> t -> list (Channel * CTree) -> CTree.
+
+  Fixpoint trOIndsOf (tr: CTree) :=
     match tr with
-    | Node i _ chd => i :: concat (map trIndicesOf chd)
+    | CNode i _ chd =>
+      i :: concat (map (fun cc => trOIndsOf (snd cc)) chd)
     end.
 
-  Definition trCurIdxOf (tr: Tree) :=
+  Definition trCurOIdxOf (tr: CTree) :=
     match tr with
-    | Node i _ _ => i
+    | CNode i _ _ => i
     end.
 
-  Definition trValueOf (tr: Tree) :=
+  Definition trValueOf (tr: CTree) :=
     match tr with
-    | Node _ v _ => v
+    | CNode _ v _ => v
     end.
 
-  Definition trChildrenOf (tr: Tree) :=
+  Definition trChildrenOf (tr: CTree) :=
     match tr with
-    | Node _ _ chd => chd
+    | CNode _ _ chd => map snd chd
     end.
 
-  Definition WfTree (tr: Tree) := NoDup (trIndicesOf tr).
+  Definition CTreeWfOInds (tr: CTree) := NoDup (trOIndsOf tr).
 
-  Fixpoint trIterate (f: Tree -> bool) (tr: Tree) :=
+  Fixpoint trIterate (f: CTree -> bool) (tr: CTree) :=
     if f tr
     then Some tr
     else match tr with
-         | Node i v chd =>
-           (fix trIterateL (trs: list Tree) :=
+         | CNode i v chd =>
+           (fix trIterateL (trs: list CTree) :=
               match trs with
               | nil => None
               | tr :: trs' =>
                 if f tr then Some tr else trIterateL trs'
-              end) chd
+              end) (map snd chd)
          end.
 
-  Fixpoint getThis (tr: Tree) (idx: IdxT): option Tree :=
+  Fixpoint getThis (tr: CTree) (idx: IdxT): option CTree :=
     trIterate (fun tr =>
-                 if trCurIdxOf tr ==n idx
+                 if trCurOIdxOf tr ==n idx
                  then true else false) tr.
 
-  Fixpoint getParent (tr: Tree) (idx: IdxT): option Tree :=
+  Fixpoint getParent (tr: CTree) (idx: IdxT): option CTree :=
     trIterate (fun tr =>
-                 if idx ?<n (map trCurIdxOf (trChildrenOf tr))
+                 if idx ?<n (map trCurOIdxOf (trChildrenOf tr))
                  then true else false) tr.
 
-  Definition getParentFwds (tr: Tree) (this: IdxT): list (IdxT * list IdxT) :=
+  Definition getParentFwds (tr: CTree) (this: IdxT): list (IdxT * list IdxT) :=
     match getThis tr this with
     | Some ttr =>
       match getParent tr this with
-      | Some ptr => (trCurIdxOf ptr, removeL eq_nat_dec (trIndicesOf tr) (trIndicesOf ttr)) :: nil
+      | Some ptr => (trCurOIdxOf ptr, removeL eq_nat_dec (trOIndsOf tr) (trOIndsOf ttr)) :: nil
       | None => nil
       end
     | None => nil
     end.
 
-  Definition getChildrenFwds (tr: Tree) (fch this: IdxT): list (IdxT * list IdxT) :=
+  Definition getChildrenFwds (tr: CTree) (fch this: IdxT): list (IdxT * list IdxT) :=
     match getThis tr this with
     | Some ttr =>
       match ttr with
-      | Node _ _ chd =>
+      | CNode _ _ chd =>
         filter (fun ii => if fst ii ==n fch then false else true)
-               (map (fun tr => (trCurIdxOf tr, trIndicesOf tr)) chd)
+               (map (fun cc => (trCurOIdxOf (snd cc), trOIndsOf (snd cc))) chd)
       end
     | None => nil
     end.
 
-  Definition getFwds (tr: Tree) (fch this: IdxT): list (IdxT * list IdxT) :=
+  Definition getFwds (tr: CTree) (fch this: IdxT): list (IdxT * list IdxT) :=
     getParentFwds tr this ++ getChildrenFwds tr fch this.
 
-End Tree.
+  Definition fromParent (tr: CTree) (this: IdxT): list IdxT := cheat _.
+  Definition isFromParent (tr: CTree) (this: IdxT) (midx: IdxT): bool := cheat _.
+  Definition fromChildren (tr: CTree) (this: IdxT): list IdxT := cheat _.
+  Definition isFromChild (tr: CTree) (this: IdxT) (midx: IdxT): bool := cheat _.
+
+End CTree.
 
